more in Compiler2.v

Compiler2.v
@@ -13,30 +13,13 @@ Fixpoint exec_n (l: list instr) (c1: config) (n: nat) (c2: config): Prop :=
     | S m => exists c', (exec1 l c1 c') /\ (exec_n l c' m c2)
   end.
 
-Definition isuccs (i: instr) (n: Z): list Z :=
+Definition isuccs (i: instr) (n: Z): list Z  :=
   match i with
     | JMP j     => [n + 1 + j]
     | JMPLESS j => [n + 1 + j; n + 1]
     | JMPGE j   => [n + 1 + j; n + 1]
     | _         => [n + 1]
   end.
-
-Definition succs (P: list instr) (n: Z)  
-                 (exprf: { i: Z |  (Z.le 0 i) /\ (Nat.lt (Z.to_nat i) (List.length P))}): list Z :=
-  isuccs (znth (proj1_sig exprf) P ADD) n.
-
-Lemma succs_empty: forall n p, succs [] n p = [].
-Proof. intros.
-       unfold succs.
-       destruct p. cbn.
-       case_eq (Z.to_nat x); intros.
-       - simpl in *.
-         destruct a. rewrite H in *.
-         contradict H1. scrush.
-       - simpl. destruct a. cbn in *.
-         rewrite H in *.
-         contradict H1. scrush.
-Qed.
 
 Definition ascii_eqb (a b: Ascii.ascii) :=
   match a, b with
@@ -74,6 +57,7 @@ Proof. intros.
        - simpl. now rewrite ascii_eqb_refl.
 Qed.
 
+
 Fixpoint instr_eqb (i1 i2: instr): bool :=
   match i1, i2 with
     | JMP i, JMP j         => Z.eqb i j
@@ -85,7 +69,6 @@ Fixpoint instr_eqb (i1 i2: instr): bool :=
     | JMPGE i, JMPGE j     => Z.eqb i j
     | _, _                 => false
   end.
-
 
 Fixpoint is_in (a: instr) (l: list instr) : bool :=
   match l with
@@ -99,19 +82,24 @@ Fixpoint is_in_Z (a: Z) (l: list Z) : bool :=
     | b :: m => Z.eqb b a || is_in_Z a m
   end.
 
-Fixpoint seqZ (start:Z) (len:nat) : list Z :=
+Definition succs (P: list instr) (n: Z)
+                 (exprf: { i: Z | (Z.le 0 i) /\ (Nat.lt (Z.to_nat i) (List.length P))}): list Z :=
+ isuccs (znth (proj1_sig exprf) P ADD) (n + (proj1_sig exprf)).
+
+Fixpoint seq (start:Z) (len:nat): list Z :=
   match len with
     | O => nil
-    | S len => start :: seqZ (Z.succ start) len
+    | S len => start :: seq (Z.succ start) len
   end.
 
-Definition _exists (P: list instr)
-                   (exprf: { i: Z | (Z.le 0 i) /\ (Nat.lt (Z.to_nat i) (List.length P))}): list Z :=
+Definition seqZ (n: Z) (m: nat) := seq n (Z.to_nat ((Z.of_nat m) - n)).
+
+Definition exits (P: list instr) exprf: list Z :=
   let l1   := succs P 0 exprf in
   let l2   := seqZ 0 (List.length P) in
-  (List.filter ( fun a => negb (is_in_Z a l1)) l2).
+  (List.filter (fun a => negb (is_in_Z a l1)) l2).
 
-Section Bop_term_exec_n.
+Section BP_term_exec_n.
 
 Lemma exec_0: forall P c, exec_n P c 0 c.
 Proof. scrush. Qed.
@@ -137,18 +125,17 @@ Proof. intros.
 		     (@Compiler.exec) (** *hammer *)].
 Qed.
 
-Lemma exec_Suc: forall n P c1 c2 c3, exec P c1 c2 -> exec_n P c2 n c3 -> exec_n P c1 (S n) c3.
-Proof. Admitted.
+Lemma exec_Suc: forall n P c1 c2 c3, exec1 P c1 c2 -> exec_n P c2 n c3 -> exec_n P c1 (S n) c3.
+Proof. intros. simpl.
+       exists c2. scrush.
+Qed.
 
 Lemma exec_exec_n: forall P c1 c2, exec P c1 c2 -> exists n, exec_n P c1 n c2.
 Proof. intros.
        induction H; intros.
        - exists O. scrush.
        - destruct IHstar as (n, IH).
-         exists (S n). apply exec_Suc with (c2 := y).
-         Focus 2. easy.
-         unfold exec. eapply star_step with (y0 := y).
-         easy. scrush.
+         exists (S n). apply exec_Suc with (c2 := y); scrush.
 Qed.
 
 Lemma exec_equiv_exec_n: forall P c1 c2, exec P c1 c2 <-> exists n, exec_n P c1 n c2.
@@ -193,46 +180,211 @@ Proof. intro k.
 		   (@Coq.Arith.PeanoNat.Nat.lt); Reconstr.scrush (** hammer *).
 Qed.
 
+
+Lemma exec1_n_step_l: forall k n n' P s s' stk stk',
+  n <> n' -> 
+  exec_n P (n, stk, s) k (n', stk', s') -> exists c, exec1 P (n, stk, s) c /\ exec_n P c (k - 1) (n', stk', s') /\ Nat.lt 0%nat k.
+Proof. intro k.
+       induction k; intros.
+       - cbn in *.
+         exists (n', stk', s'); scrush.
+       - cbn in *. destruct H0. exists x.
+         destruct H0. split. scrush.
+         split. scrush.
+	       Reconstr.htrivial Reconstr.Empty
+		     (@Coq.Arith.PeanoNat.Nat.lt_0_succ)
+		     (@Coq.Arith.PeanoNat.Nat.lt); scrush.
+Qed.
+
+
 Lemma exec_n_step_r: forall k n n' P s s' stk stk',
   n <> n' -> 
-  (exists c, exec P (n, stk, s) c /\ exec_n P c (k - 1) (n', stk', s') /\ Nat.lt 0%nat k) -> exec_n P (n, stk, s) k (n', stk', s').
+  (exists c, exec1 P (n, stk, s) c /\ exec_n P c (k - 1) (n', stk', s') /\ Nat.lt 0%nat k) ->
+   exec_n P (n, stk, s) k (n', stk', s').
 Proof. intros.
        case_eq k; intros.
        - destruct H0, H0, H2. subst.
          contradict H3. scrush.
        - simpl. destruct H0, H0, H2.
-         eapply (exec_Suc) with (n := n0) (c3 := (n', stk', s')) in H0.
-         cbn in *. destruct H0.
-         exists x0. easy. 
+         exists x. split. easy.
          assert ((S n0 - 1)%nat = n0) by scrush. subst.
          now rewrite <- H4.
 Qed.
 
-End Bop_term_exec_n.
+End BP_term_exec_n.
 
 Section CSES.
 
 Lemma exec_n_step: forall k n n' P s s' stk stk',
   n <> n' ->
-  (exists c, exec P (n, stk, s) c /\ exec_n P c (k - 1) (n', stk', s') /\ Nat.lt 0%nat k) <-> 
+  (exists c, exec1 P (n, stk, s) c /\ exec_n P c (k - 1) (n', stk', s') /\ Nat.lt 0%nat k) <-> 
   exec_n P (n, stk, s) k (n', stk', s').
 Proof. split; intros. 
        pose exec_n_step_r; scrush.
-       pose exec_n_step_l; scrush.
+       pose exec1_n_step_l; scrush.
 Qed.
 
-Lemma exec1_end: forall P c1 c2, size P <= (fst (fst c1)) -> (exec P c1 c2 -> False).
+Lemma execn_end: forall k n n' P s s' stk stk',
+  size P <= n -> exec_n P (n, s, stk) k (n', s', stk') -> (n' = n /\ stk' = stk /\ s' = s /\ k = 0%nat).
+Proof. intro k.
+       induction k; intros.
+       - cbn in *; scrush.
+       - cbn in *.
+         destruct H0, H0.
+	       Reconstr.hcrush (@H0, @H)
+		        (@Coq.ZArith.BinInt.Z.lt_nge, @Coq.ZArith.BinInt.Z.gt_lt_iff)
+		        Reconstr.Empty.
+Qed.
+
+
+Lemma exec1_end: forall P c1 c2, size P <= (fst (fst c1)) -> (exec1 P c1 c2 -> False).
+Proof. intros.
+       destruct c1, p.
+       cbn in *. unfold exec1 in *.
+       destruct H0, H0, H0, H0.
+       inversion H0. subst.
+       destruct H1, H2.
+       assert ((size P <= x) -> (x < size P) -> False).
+       { Reconstr.hobvious (@H, @H3)
+	       (@Coq.ZArith.BinInt.Z.lt_nge)
+		     Reconstr.Empty.
+       } scrush.
+Qed.
+
+End CSES.
+
+Section BP_term_succs.
+
+Lemma succs_simps: forall n v x i p, succs [ADD] n p       = [n + 1]            /\
+                                     succs [LOADI v] n p   = [n + 1]            /\
+                                     succs [LOAD x] n p    = [n + 1]            /\
+                                     succs [STORE x] n p   = [n + 1]            /\
+                                     succs [JMP i] n p     = [n + 1 + i]        /\
+                                     succs [JMPGE i] n p   = [n + 1 + i; n + 1] /\
+                                     succs [JMPLESS i] n p = [n + 1 + i; n + 1].
+Proof. intros; destruct p; 
+       unfold succs; cbn in *;
+       destruct a;
+       assert (x0 = 0).
+	     { Reconstr.htrivial (@H, @H0)
+		    (@Coq.ZArith.BinInt.Z.lt_succ_r, @Coq.ZArith.BinInt.Z.le_refl, 
+         @Coq.ZArith.BinInt.Z.le_antisymm, @Coq.ZArith.BinInt.Z.log2_up_nonpos, 
+         @Coq.ZArith.BinInt.Z.log2_up_null, @Coq.ZArith.Znat.Z2Nat.inj_0, 
+         @Coq.ZArith.Znat.Z2Nat.inj_succ, @Coq.ZArith.Znat.Z2Nat.inj_lt,
+         @Coq.ZArith.BinInt.Z.one_succ) (@Coq.Arith.PeanoNat.Nat.lt); scrush.
+        } scrush.
+Qed.
+
+Lemma succs_empty: forall n p, succs [] n p = [].
+Proof. intros; destruct p; scrush. Qed.
+
+Lemma prf_cons: forall (x: instr) (xs: list instr), 
+{i : Z | 0 <= i /\ Nat.lt (Z.to_nat i) (List.length xs)} -> 
+{i : Z | 0 <= i /\ Nat.lt (Z.to_nat i) (List.length (x :: xs))}.
+Proof. intros. destruct H. exists x0. scrush. Defined. 
+
+Lemma succs_Cons: forall x xs n p,
+NoDup (succs (x :: xs) n (prf_cons x xs p)) ->
+NoDup ((isuccs x n ++ succs xs (n + 1) p)) ->
+succs (x :: xs) n (prf_cons x xs p) = (isuccs x n ++ succs xs (n + 1) p).
 Proof. Admitted.
 
+Lemma succs_iexec1: forall P s stk c p, 
+                                        c = iexec (znth (proj1_sig p) P ADD) ((proj1_sig p), s, stk) ->
+                                        List.In (fst (fst c)) (succs P 0 p).
+Proof. intros; destruct c, p0, p; unfold succs, isuccs; scrush. Qed.
 
+
+Lemma In_Singleton: forall {A} (a b: A),  In a [b] -> a = b.
+Proof. intros; destruct H; cbn in *; scrush. Qed.
+
+Lemma succs_shift: forall P n k p, List.In (k - n) (succs P 0 p) -> List.In k (succs P n p).
+Proof. intros.
+       destruct p. cbn in *.
+       unfold succs in *. cbn in *.
+       unfold isuccs in *.
+       case_eq (znth x P ADD ); intros; rewrite H0 in *.
+       apply In_Singleton in H.
+       assert (k = n + x + 1).
+       { 	Reconstr.htrivial (@H)
+		     (@Coq.ZArith.BinInt.Zplus_assoc_reverse, @Coq.ZArith.BinInt.Zplus_minus)
+		      Reconstr.Empty.
+       } scrush.
+       apply In_Singleton in H.
+       assert (k = n + x + 1).
+       { 	Reconstr.htrivial (@H)
+		     (@Coq.ZArith.BinInt.Zplus_assoc_reverse, @Coq.ZArith.BinInt.Zplus_minus)
+		      Reconstr.Empty.
+       } scrush.
+       apply In_Singleton in H.
+       assert (k = n + x + 1).
+       { 	Reconstr.htrivial (@H)
+		     (@Coq.ZArith.BinInt.Zplus_assoc_reverse, @Coq.ZArith.BinInt.Zplus_minus)
+		      Reconstr.Empty.
+       } scrush.
+       apply In_Singleton in H.
+       assert (k = n + x + 1).
+       { 	Reconstr.htrivial (@H)
+		     (@Coq.ZArith.BinInt.Zplus_assoc_reverse, @Coq.ZArith.BinInt.Zplus_minus)
+		      Reconstr.Empty.
+       } scrush.
+       apply In_Singleton in H.
+       assert (k = n + x + 1 + z).
+       { Reconstr.htrivial (@H)
+		     (@Coq.ZArith.BinInt.Zplus_assoc_reverse, @Coq.ZArith.BinInt.Z.add_simpl_r, @Coq.ZArith.BinInt.Zplus_minus)
+		     Reconstr.Empty.
+       } scrush.
+       inversion H.
+       assert (k = n + x + 1 + z).
+       { Reconstr.htrivial (@H1)
+		     (@Coq.ZArith.BinInt.Zplus_minus, @Coq.ZArith.BinInt.Zplus_assoc_reverse)
+		     Reconstr.Empty.
+       } scrush.
+       apply In_Singleton in H1.
+       assert (k = n + x + 1).
+       { Reconstr.htrivial (@H1)
+		     (@Coq.ZArith.BinInt.Zplus_minus, @Coq.ZArith.BinInt.Zplus_assoc_reverse)
+		     Reconstr.Empty.
+       } scrush.
+       inversion H.
+       assert (k = n + x + 1 + z).
+       { Reconstr.htrivial (@H1)
+		     (@Coq.ZArith.BinInt.Zplus_minus, @Coq.ZArith.BinInt.Zplus_assoc_reverse)
+		     Reconstr.Empty.
+       } scrush.
+       apply In_Singleton in H1.
+       assert (k = n + x + 1).
+       { Reconstr.htrivial (@H1)
+		     (@Coq.ZArith.BinInt.Zplus_minus, @Coq.ZArith.BinInt.Zplus_assoc_reverse)
+		     Reconstr.Empty.
+       } scrush.
+Qed.
+
+Lemma acomp_succs: forall a (n: Z) p, succs (acomp a) n p = seqZ n (Z.to_nat n + (List.length (acomp a))).
+Proof. Admitted.
+
+Lemma helper: forall (xs ys: list instr) a,
+Nat.lt (Z.to_nat a) (Datatypes.length ys) ->
+Nat.lt (Z.to_nat a) (Datatypes.length (xs ++ ys)).
+Proof. intro xs.
+       induction xs; intros.
+       - now cbn.
+       - simpl. scrush.
+Qed.
+
+Lemma prf_concat: forall (xs ys: list instr),
+{i : Z | 0 <= i /\ Nat.lt (Z.to_nat i) (Datatypes.length ys)} ->
+{i : Z | 0 <= i /\ Nat.lt (Z.to_nat i) (Datatypes.length (xs ++ ys))}. 
+Proof. intros. destruct H. exists x. split. easy.
+       destruct a. now apply helper.
+Defined.  
+
+Lemma succs_append: forall xs ys n p q, succs (xs ++ ys) n (prf_concat xs ys p) = succs xs n q ++ succs ys (n + size xs) p.
+Proof. Admitted.
 
 (** go through the whole file..! *)
 
 
-End CSES.
-
-
-
-
+End BP_term_succs.
 
 
